---
title: "メビウス関数の和"
---


[[メビウス関数]]の和
$ \sum_{d|n}\mu (d)=\left\{ \begin{array} {l}1 &(n=1) \\ 0 & (n>1)\end{array} \right.$


- $\sum_{k=0}^n (-1)^k \binom{n}{k} = 0$
    - [[二項定理]]
        - $(-1 + 1) ^ n = \sum_{k=0}^n (-1)^k 1^{n-k} \binom{n}{k} = \sum_{k=0}^n (-1)^k \binom{n}{k}$
        - $(-1 + 1) ^ n = 0^n = 0$

$\sum_{d|n} \mu(n/d) g(d) = \sum_{d|n} \mu(n/d) \sum_{l|d} f(l) = \sum_{d|n} \sum_{l|d} \mu(n/d)  f(l)$

$\sum_{d|n} \sum_{l|d} \mu(n/d)  f(l) = \sum_{l|n} f(l) \sum_{(n/d)|(n/l)} \mu(n/d)$

eq1より
$\sum_{(n/d)|(n/l)} \mu(n/d) =\left\{ \begin{array} {l}1 &(n/l=1) \\ 0 & (n/l>1)\end{array} \right.$


- [メビウスの反転公式と3つの応用 - 数学とその他の日々](http://br-h2gk.hatenablog.com/entry/mebius_01)
from [[ゼータ変換/メビウス変換20201105]]
