
行列Aが対称である時
$\sum_{i=1}^{N-1} \sum_{j=i+1}^N A_{ij} = \left(\sum_{ij} A_{ij} - \sum_i A_{ii}\right) / 2$
- 具体例 [[ABC177C]]
    - $A_{ij} = A_iA_j$ のとき$\sum_{i=1}^{N-1} \sum_{j=i+1}^N A_iA_j = \left(\sum_{ij} A_iA_j - \sum_i A_i^2\right) / 2$
        - なお$\sum_{ij} A_iA_j = \left(\sum A_i\right)^2$

特に対角成分が0の時
- $\sum_{i=1}^{N-1} \sum_{j=i+1}^N A_{ij} = \left(\sum_{ij} A_{ij}\right) / 2$
- 具体例 [[ABC194]]C
    - $A_{ij} = (A_i - A_j)^2$ のとき $\sum_{i=1}^{N-1} \sum_{j=i+1}^N A_{ij} = \left(\sum_{ij} (A_i - A_j)^2 \right) / 2$
- [[ABC147D]]
    - $A_{ij} = A_i \oplus A_j$
